ironfleet/src/Dafny/Distributed/Impl/Common/CmdLineParser.i.dfy
@@ -11,151 +11,18 @@ import opened Math__power_s
 import opened Common__SeqIsUniqueDef_i
 import opened Common__NetClient_i
 
-function method ascii_to_int(short:uint16) : (bool, byte)
-  ensures var tuple := ascii_to_int(short);
-          tuple.0 ==> 0 <= tuple.1 <= 9
-{
-  if 48 <= short <= 57 then
-    (true, (short - 48) as byte)
-  else 
-    (false, 0)
-}
-
-method power10(e:nat) returns (val:int)
-  ensures val == power(10, e)
-{
-  reveal power();
-  if e == 0 {
-    return 1;
-  } else {
-    var tmp := power10(e-1);
-    return 10 * tmp;
-  }
-}
-
-function method shorts_to_bytes(shorts:seq<uint16>) : (bool, seq<byte>)
-{
-  if |shorts| == 0 then (true, [])
-  else 
-    var tuple := shorts_to_bytes(shorts[1..]);
-    var ok, rest := tuple.0, tuple.1;
-    var tuple' := ascii_to_int(shorts[0]);
-    var ok', a_byte := tuple'.0, tuple'.1;
-    if ok && ok' then
-      (true, [a_byte] + rest)
-    else
-      (false, [])
-}
-
-function method bytes_to_decimal(bytes:seq<byte>) : nat
-{
-  if |bytes| == 0 then 0
-  else (bytes[|bytes|-1] as int) + 10 * bytes_to_decimal(bytes[0..|bytes|-1])
-}
-
-function method shorts_to_nat(shorts:seq<uint16>) : (bool, int)
-{
-  if |shorts| == 0 then (false, 0)
-  else 
-    var tuple := shorts_to_bytes(shorts);
-    var ok, bytes := tuple.0, tuple.1;
-    if !ok then (false, 0)
-    else
-      (true, bytes_to_decimal(bytes))
-}
-
-function method shorts_to_byte(shorts:seq<uint16>) : (bool, byte)
-{
-  var tuple := shorts_to_nat(shorts);
-  var ok, val := tuple.0, tuple.1;
-  if 0 <= val < 0x100 then
-    (true, val as byte)
-  else
-    (false, 0)
-}
-
-function method shorts_to_uint16(shorts:seq<uint16>) : (bool, uint16)
-{
-  var tuple := shorts_to_nat(shorts);
-  var ok, val := tuple.0, tuple.1;
-  if 0 <= val < 0x10000 then
-    (true, val as uint16)
-  else
-    (false, 0)
-}
-
-function method shorts_to_uint32(shorts:seq<uint16>) : (bool, uint32)
-{
-  var tuple := shorts_to_nat(shorts);
-  var ok, val := tuple.0, tuple.1;
-  if 0 <= val < 0x1_0000_0000 then
-    (true, val as uint32)
-  else
-    (false, 0)
-}
-
-function method is_ascii_period(short:uint16) : (bool)
-{
-  short == 46
-}
-
-function method parse_ip_addr_helper(ip_shorts:seq<uint16>, current_octet_shorts:seq<uint16>) : (bool, seq<byte>)
-{
-  if |ip_shorts| == 0 then 
-    var tuple := shorts_to_byte(current_octet_shorts);
-    var okay, b := tuple.0, tuple.1;
-    if !okay then (false, []) else (true, [b])
-  else
-    if is_ascii_period(ip_shorts[0]) then
-      var tuple := shorts_to_byte(current_octet_shorts);
-      var okay, b := tuple.0, tuple.1;
-      if !okay then
-        (false, [])
-      else
-        var tuple' := parse_ip_addr_helper(ip_shorts[1..], []);
-        var ok, ip_bytes := tuple'.0, tuple'.1;
-        if !ok then
-          (false, [])
-        else
-          (true, [b] + ip_bytes)
-    else
-      parse_ip_addr_helper(ip_shorts[1..], current_octet_shorts + [ip_shorts[0]])
-}
-
-function method parse_ip_addr(ip_shorts:seq<uint16>) : (bool, seq<byte>)
-{
-  var tuple := parse_ip_addr_helper(ip_shorts, []);
-  var ok, ip_bytes := tuple.0, tuple.1;
-  if ok && |ip_bytes| == 4 then
-    (true, ip_bytes)
-  else 
-    (false, [])
-}
-
-
-function method {:opaque} parse_end_point(ip_shorts:seq<uint16>, port_shorts:seq<uint16>) : (bool, EndPoint)
-  ensures var tuple := parse_end_point(ip_shorts,port_shorts);
+function method parse_end_point(public_key:seq<byte>) : (bool, EndPoint)
+  ensures var tuple := parse_end_point(public_key);
           var ok, ep := tuple.0, tuple.1;
-          ok ==> EndPointIsValidIPV4(ep)
+          ok ==> EndPointIsValidPublicKey(ep)
 {
-  var tuple := parse_ip_addr(ip_shorts);
-  var okay, ip_bytes := tuple.0, tuple.1;
-
-  if !okay then 
-    //print("Failed to parse_ip_addr\n");
-    (false, EndPoint([0,0,0,0], 0))
+  if |public_key| < 0x10_0000 then
+    (true, EndPoint(public_key))
   else
-    var tuple' := shorts_to_uint16(port_shorts);
-    var okay', port := tuple'.0, tuple'.1;
-    if !okay' then 
-      //print("Failed to parse port\n");
-      (false, EndPoint([0,0,0,0], 0))
-    else
-      (true, EndPoint(ip_bytes, port))
-
+    (false, EndPoint(public_key))
 }
 
-method test_unique'(endpoints:seq<EndPoint>) returns (unique:bool)
+method test_unique(endpoints:seq<EndPoint>) returns (unique:bool)
   ensures unique <==> SeqIsUnique(endpoints)
 {
   unique := true;
@@ -184,16 +51,15 @@ method test_unique'(endpoints:seq<EndPoint>) returns (unique:bool)
   reveal SeqIsUnique();
 }
 
-function method parse_end_points(args:seq<seq<uint16>>) : (bool, seq<EndPoint>)
-  requires |args| % 2 == 0
+function method parse_end_points(args:seq<seq<byte>>) : (bool, seq<EndPoint>)
   ensures var (ok, endpoints) := parse_end_points(args);
-          ok ==> (forall e :: e in endpoints ==> EndPointIsValidIPV4(e))
+          ok ==> (forall e :: e in endpoints ==> EndPointIsValidPublicKey(e))
 {
   if |args| == 0 then
     (true, [])
   else
-    var (ok1, ep) := parse_end_point(args[0], args[1]);
-    var (ok2, rest) := parse_end_points(args[2..]);
+    var (ok1, ep) := parse_end_point(args[0]);
+    var (ok2, rest) := parse_end_points(args[1..]);
 
     if !(ok1 && ok2) then
       (false, [])
@@ -201,7 +67,7 @@ function method parse_end_points(args:seq<seq<uint16>>) : (bool, seq<EndPoint>)
       (true, [ep] + rest)
 }
 
-method collect_cmd_line_args(ghost env:HostEnvironment) returns (args:seq<seq<uint16>>)
+method collect_cmd_line_args(ghost env:HostEnvironment) returns (args:seq<seq<byte>>)
   requires HostEnvironmentIsValid(env)
   ensures  |env.constants.CommandLineArgs()| == |args|
   ensures  forall i :: 0 <= i < |env.constants.CommandLineArgs()| ==> args[i] == env.constants.CommandLineArgs()[i]
@@ -219,51 +85,6 @@ method collect_cmd_line_args(ghost env:HostEnvironment) returns (args:seq<seq<ui
     args := args + [arg[..]];
     i := i + 1;
   }
-}
-
-// "foo:bar:10 --> ("foo:bar", "10")
-// "foo" -> ("foo", "")
-function method split_at_last_colon(str:seq<uint16>, n:nat) : (seq<uint16>, seq<uint16>)
-  requires n <= |str|
-{
-  if n == 0 then
-    (str, [])
-  else if str[n - 1] == ':' as uint16 then
-    (str[.. n - 1], str[n ..])
-  else
-    split_at_last_colon(str, n - 1)
-}
-
-function method resolve_ip_address(str:seq<uint16>) : (seq<uint16>)
-{
-  if parse_ip_addr(str).0 then
-    // already an IP address
-    str
-  else
-    // resolve
-    IPEndPoint.DnsResolve(str)
-}
-
-function method resolve_cmd_line_args_rec(args:seq<seq<uint16>>) : (args':seq<seq<uint16>>)
-  ensures |args'| >= |args|
-{
-  if |args| == 0 then
-    args
-  else
-    var (s1, s2) := split_at_last_colon(args[0], |args[0]|);
-    if |s2| == 0 then
-      [s1] + resolve_cmd_line_args_rec(args[1..])
-    else
-      [resolve_ip_address(s1), s2] + resolve_cmd_line_args_rec(args[1..])
-}
-
-function method resolve_cmd_line_args(args:seq<seq<uint16>>) : (args':seq<seq<uint16>>)
-  ensures |args'| >= |args|
-{
-  if |args| == 0 then
-    args
-  else
-    [args[0]] + resolve_cmd_line_args_rec(args[1..])
 }
 
 }
