ironfleet/src/Dafny/Distributed/Common/Framework/Host.s.dfy
@@ -20,10 +20,7 @@ predicate HostStateInvariants(host_state:HostState, env:HostEnvironment)
   reads *
 predicate ConcreteConfigurationInvariants(config:ConcreteConfiguration)
 
-function ResolveCommandLine(args:seq<seq<uint16>>) : (args':seq<seq<uint16>>)
-  ensures |args'| >= |args|
-function ParseCommandLineConfiguration(args:seq<seq<uint16>>) : (ConcreteConfiguration, set<EndPoint>, set<EndPoint>)
-function ParseCommandLineId(ip:seq<uint16>, port:seq<uint16>) : EndPoint
+function ParseCommandLineConfiguration(args:seq<seq<byte>>) : (ConcreteConfiguration, set<EndPoint>, set<EndPoint>)
 
 predicate ArbitraryObject(o:object) { true }
 
@@ -44,15 +41,14 @@ method HostInitImpl(ghost env:HostEnvironment) returns (
   ensures  ok ==> |env.constants.CommandLineArgs()| >= 2
   ensures  ok ==> HostStateInvariants(host_state, env)
   ensures  ok ==> ConcreteConfigurationInvariants(config)
-  ensures  ok ==> var args := ResolveCommandLine(env.constants.CommandLineArgs());
-                  var (parsed_config, parsed_servers, parsed_clients) := ParseCommandLineConfiguration(args[0..|args|-2]);
+  ensures  ok ==> var args := env.constants.CommandLineArgs();
+                  var (parsed_config, parsed_servers, parsed_clients) := ParseCommandLineConfiguration(args[0..|args|-1]);
                   && config == parsed_config
                   && servers == parsed_servers
                   && clients == parsed_clients
-                  && ConcreteConfigInit(parsed_config, parsed_servers, parsed_clients);
-  ensures  ok ==> var args := ResolveCommandLine(env.constants.CommandLineArgs());
-                  && id == ParseCommandLineId(args[|args|-2], args[|args|-1])
-                  && HostInit(host_state, config, id);
+                  && ConcreteConfigInit(parsed_config, parsed_servers, parsed_clients)
+                  && id == EndPoint(args[|args|-1])
+                  && HostInit(host_state, config, id)
 
 method HostNextImpl(ghost env:HostEnvironment, host_state:HostState) 
   returns (
