ironfleet/src/Dafny/Distributed/Impl/LiveSHT/CmdLineParser.i.dfy
@@ -11,142 +11,142 @@ import opened Common__NetClient_i
 import opened Common__SeqIsUniqueDef_i
 import opened Common__NodeIdentity_i
 
-function method EndPointNull() : EndPoint { EndPoint([0, 0, 0, 0], 0) }
+function EndPointNull () : EndPoint
+{
+  EndPoint([])
+}
 
 function ConstantsStateNull () : ConstantsState 
 {
-    ConstantsState(EndPointNull(), [], StaticParams())
+  ConstantsState(EndPointNull(), [], StaticParams())
 }
 
-function sht_config_parsing(args:seq<seq<uint16>>) : ConstantsState
+function sht_config_parsing(args:seq<seq<byte>>) : ConstantsState
 {
-    if args != [] && |args[1..]| % 2 == 0 then 
-        var (ok, endpoints) := parse_end_points(args[1..]);
-        ConstantsState(if |endpoints| > 0 then endpoints[0] else EndPointNull(), // Root is the first endpoint in the list
-                       endpoints,
-                       StaticParams())
-    else 
-        ConstantsStateNull()
+  var (ok, endpoints) := parse_end_points(args);
+  if !ok then
+    ConstantsStateNull()
+  else
+    ConstantsState(if |endpoints| > 0 then endpoints[0] else EndPointNull(), // Root is the first endpoint in the list
+                   endpoints,
+                   StaticParams())
 }
 
-function sht_parse_id(ip:seq<uint16>, port:seq<uint16>) : EndPoint
+function sht_parse_id(arg:seq<byte>) : EndPoint
 {
-    var (ok, ep) := parse_end_point(ip, port);
-    ep
+  var (ok, ep) := parse_end_point(arg);
+  ep
 }
 
 function sht_cmd_line_parsing(env:HostEnvironment) : (ConstantsState, EndPoint)
-    reads env;
-    reads env.constants;
+  reads env
+  reads env.constants
 {
-    var args := resolve_cmd_line_args(env.constants.CommandLineArgs());
-    if |args| < 2 then
-        (ConstantsStateNull(), EndPointNull()) 
-    else
-        var penultimate_arg, final_arg := args[|args|-2], args[|args|-1];
-        var config := sht_config_parsing(args[..|args|-2]);
-        var me := sht_parse_id(penultimate_arg, final_arg);
-        (config, me)
+  var args := env.constants.CommandLineArgs();
+  if |args| < 1 then
+    (ConstantsStateNull(), EndPointNull()) 
+  else
+    var final_arg := args[|args|-1];
+    var config := sht_config_parsing(args[..|args|-1]);
+    var me := sht_parse_id(final_arg);
+    (config, me)
 }
 
 method GetHostIndex(host:EndPoint, hosts:seq<EndPoint>) returns (found:bool, index:uint64)
-    requires EndPointIsValidIPV4(host);
-    requires SeqIsUnique(hosts);
-    requires |hosts| < 0x1_0000_0000_0000_0000;
-    requires forall h :: h in hosts ==> EndPointIsValidIPV4(h);
-    ensures  found ==> 0 <= index as int < |hosts| && hosts[index] == host;
-    ensures !found ==> !(host in hosts);
-    ensures !found ==> !(AbstractifyEndPointToNodeIdentity(host) in AbstractifyEndPointsToNodeIdentities(hosts));
+  requires EndPointIsValidPublicKey(host)
+  requires SeqIsUnique(hosts)
+  requires |hosts| < 0x1_0000_0000_0000_0000
+  requires forall h :: h in hosts ==> EndPointIsValidPublicKey(h)
+  ensures  found ==> 0 <= index as int < |hosts| && hosts[index] == host
+  ensures !found ==> !(host in hosts)
+  ensures !found ==> !(AbstractifyEndPointToNodeIdentity(host) in AbstractifyEndPointsToNodeIdentities(hosts))
 {
-    var i:uint64 := 0;
-    lemma_AbstractifyEndPointsToNodeIdentities_properties(hosts);
+  var i:uint64 := 0;
+  lemma_AbstractifyEndPointsToNodeIdentities_properties(hosts);
 
-    while i < |hosts| as uint64
-        invariant i as int <= |hosts|;
-        invariant forall j :: 0 <= j < i ==> hosts[j] != host;
-    {
-        if host == hosts[i] {
-            found := true;
-            index := i;
+  while i < |hosts| as uint64
+    invariant i as int <= |hosts|;
+    invariant forall j :: 0 <= j < i ==> hosts[j] != host;
+  {
+    if host == hosts[i] {
+      found := true;
+      index := i;
     
-            calc ==> {
-                true;
-                    { reveal_SeqIsUnique(); }
-                forall j :: 0 <= j < |hosts| && j != i as int ==> hosts[j] != host;
-            }
+      calc ==> {
+        true;
+          { reveal_SeqIsUnique(); }
+        forall j :: 0 <= j < |hosts| && j != i as int ==> hosts[j] != host;
+      }
 
-            return;
-        }
-
-        if i == |hosts| as uint64 - 1 {
-            found := false;
-            return;
-        }
-
-        i := i + 1;
+      return;
     }
-    found := false;
+
+    if i == |hosts| as uint64 - 1 {
+      found := false;
+      return;
+    }
+
+    i := i + 1;
+  }
+  found := false;
 }
 
 method parse_cmd_line(ghost env:HostEnvironment) returns (ok:bool, config:ConstantsState, my_index:uint64)
-    requires HostEnvironmentIsValid(env);
-    ensures ok ==> ConstantsStateIsValid(config);
-    ensures ok ==> |config.hostIds| > 0;
-    ensures ok ==> 0 <= my_index as int < |config.hostIds|;
-    //ensures (config, my_index) == sht_cmd_line_parsing(env);
-    ensures var (config', my_ep') := sht_cmd_line_parsing(env);
-            ok ==> config == config' && config.hostIds[my_index] == my_ep';
+  requires HostEnvironmentIsValid(env)
+  ensures ok ==> ConstantsStateIsValid(config)
+  ensures ok ==> |config.hostIds| > 0
+  ensures ok ==> 0 <= my_index as int < |config.hostIds|
+  //ensures (config, my_index) == sht_cmd_line_parsing(env)
+  ensures var (config', my_ep') := sht_cmd_line_parsing(env);
+          ok ==> config == config' && config.hostIds[my_index] == my_ep'
 {
+  ok := false;
+  var num_args := HostConstants.NumCommandLineArgs(env);
+  var args := collect_cmd_line_args(env);
+  assert args == env.constants.CommandLineArgs();
+
+  if |args| < 2 {
+    print "Incorrect number of command line arguments.\n";
+    print "Expected: ./Main.exe [public_key]+ [public_key]\n";
+    print "  where the final argument is one of the public keys provided earlier \n";
+    print "Note that the first public key indicates the root identity\n";
+    return;
+  }
+
+  var tuple1 := parse_end_points(args[..|args|-1]);
+  ok := tuple1.0;
+  var endpoints := tuple1.1;
+  if !ok || |endpoints| >= 0xffff_ffff_ffff_ffff {
     ok := false;
-    var num_args := HostConstants.NumCommandLineArgs(env);
-    var args := collect_cmd_line_args(env);
-    assert args == env.constants.CommandLineArgs();
+    return;
+  }
 
-    args := resolve_cmd_line_args(args);
+  var tuple2 := parse_end_point(args[|args|-1]);
+  ok := tuple2.0;
+  if !ok {
+    return;
+  }
 
-    if |args| < 4 || |args| % 2 != 1 {
-        print "Incorrect number of command line arguments.\n";
-        print "Expected: ./Main.exe [name:port]+ [name:port]\n";
-        print "      or: ./Main.exe [IP port]+ [IP port]\n";
-        print "  where the final argument is one of the IP-port pairs provided earlier \n";
-        print "Note that the first IP-port pair indicates the root identity\n";
-        return;
-    }
+  var unique := test_unique(endpoints);
+  if !unique {
+    ok := false;
+    return;
+  }
 
-    var tuple1 := parse_end_points(args[1..|args|-2]);
-    ok := tuple1.0;
-    var endpoints := tuple1.1;
-    if !ok || |endpoints| >= 0xffff_ffff_ffff_ffff {
-        ok := false;
-        return;
-    }
+  ok, my_index := GetHostIndex(tuple2.1, endpoints);
+  if !ok {
+    return;
+  }
+  var root_identity := endpoints[0];
+  var hosts := endpoints;
+  var me := endpoints[my_index];
 
-    var tuple2 := parse_end_point(args[|args|-2], args[|args|-1]);
-    ok := tuple2.0;
-    if !ok {
-        return;
-    }
+  config := ConstantsState(root_identity, hosts, StaticParams());
 
-    var unique := test_unique'(endpoints);
-    if !unique {
-        ok := false;
-        return;
-    }
-
-    ok, my_index := GetHostIndex(tuple2.1, endpoints);
-    if !ok {
-        return;
-    }
-    var root_identity := endpoints[0];
-    var hosts := endpoints;
-    var me := endpoints[my_index];
-
-    config := ConstantsState(root_identity, hosts, StaticParams());
-
-    ghost var ghost_tuple := sht_cmd_line_parsing(env);
-    ghost var config', my_ep' := ghost_tuple.0, ghost_tuple.1;
-    assert endpoints == config'.hostIds;
-    assert config == config';
-    assert me == my_ep';
+  ghost var ghost_tuple := sht_cmd_line_parsing(env);
+  ghost var config', my_ep' := ghost_tuple.0, ghost_tuple.1;
+  assert endpoints == config'.hostIds;
+  assert config == config';
+  assert me == my_ep';
 }
 }
